Renamed lvalue / hom -> register / preregister

Axioms_Classical.thy
@@ -1,10 +1,10 @@
-section \<open>Classical instantiation of lvalues\<close>
+section \<open>Classical instantiation of registerss\<close>
 
 (* AXIOM INSTANTIATION (use instantiate_laws.py to generate Laws_Classical.thy)
  
    domain \<rightarrow> type
 
-   Generic laws about lvalues \<rightarrow> Generic laws about lvalues, instantiated classically
+   Generic laws about registers \<rightarrow> Generic laws about registers, instantiated classically
 *)
 
 theory Axioms_Classical
@@ -27,41 +27,41 @@ lemma id_update_right: "comp_update a id_update = a"
 lemma comp_update_assoc: "comp_update (comp_update a b) c = comp_update a (comp_update b c)"
   by auto
 
-type_synonym ('a,'b) update_hom = \<open>'a update \<Rightarrow> 'b update\<close>
-definition update_hom :: \<open>('a,'b) update_hom \<Rightarrow> bool\<close> where
-  \<open>update_hom F \<longleftrightarrow> (\<exists>R. F = Image R)\<close>
+type_synonym ('a,'b) preregister = \<open>'a update \<Rightarrow> 'b update\<close>
+definition preregister :: \<open>('a,'b) preregister \<Rightarrow> bool\<close> where
+  \<open>preregister F \<longleftrightarrow> (\<exists>R. F = Image R)\<close>
 
-lemma id_update_hom: \<open>update_hom id\<close>
-  unfolding update_hom_def
+lemma id_preregister: \<open>preregister id\<close>
+  unfolding preregister_def
   by (metis Image_Id eq_id_iff)
 
-lemma update_hom_mult_right: \<open>update_hom (\<lambda>a. comp_update a z)\<close>
-  unfolding update_hom_def 
+lemma preregister_mult_right: \<open>preregister (\<lambda>a. comp_update a z)\<close>
+  unfolding preregister_def 
   apply (rule exI[of _ \<open>{((a,b),(c,b))| a b c. (c,a) \<in> z}\<close>])
   by (auto intro!:ext simp: relcomp_def relcompp_apply Image_def[abs_def])
 
-lemma update_hom_mult_left: \<open>update_hom (\<lambda>a. comp_update z a)\<close>
-  unfolding update_hom_def 
+lemma preregister_mult_left: \<open>preregister (\<lambda>a. comp_update z a)\<close>
+  unfolding preregister_def 
   apply (rule exI[of _ \<open>{((a,b),(a,d))| a b c d. (b,d) \<in> z}\<close>])
   by (auto intro!:ext simp: relcomp_def relcompp_apply Image_def[abs_def])
 
-definition rel_of_update_hom :: \<open>('a,'b) update_hom \<Rightarrow> (('a\<times>'a)\<times>('b\<times>'b)) set\<close> where
-  \<open>rel_of_update_hom F = (SOME R. F = Image R)\<close>
+definition rel_of_preregister :: \<open>('a,'b) preregister \<Rightarrow> (('a\<times>'a)\<times>('b\<times>'b)) set\<close> where
+  \<open>rel_of_preregister F = (SOME R. F = Image R)\<close>
 
-lemma rel_of_update_hom: \<open>update_hom F \<Longrightarrow> F = Image (rel_of_update_hom F)\<close>
-  unfolding update_hom_def rel_of_update_hom_def
+lemma rel_of_preregister: \<open>preregister F \<Longrightarrow> F = Image (rel_of_preregister F)\<close>
+  unfolding preregister_def rel_of_preregister_def
   by (metis (mono_tags) someI_ex)
 
-lemma update_hom_mono: "update_hom F \<Longrightarrow> mono F"
-  by (auto simp: update_hom_def mono_def Image_def)
+lemma preregister_mono: "preregister F \<Longrightarrow> mono F"
+  by (auto simp: preregister_def mono_def Image_def)
 
-lemma comp_update_hom: "update_hom F \<Longrightarrow> update_hom G \<Longrightarrow> update_hom (G \<circ> F)"
-  unfolding update_hom_def apply auto
+lemma comp_preregister: "preregister F \<Longrightarrow> preregister G \<Longrightarrow> preregister (G \<circ> F)"
+  unfolding preregister_def apply auto
   apply (rule_tac x=\<open>R O Ra\<close> in exI)
   by (auto simp: o_def)
 
-lemma converse_hom: \<open>update_hom converse\<close>
-  unfolding update_hom_def
+lemma converse_preregister: \<open>preregister converse\<close>
+  unfolding preregister_def
   apply (rule exI[where x=\<open>{((x,y),(y,x))| x y. True}\<close>])
   by (auto simp: converse_def Image_def)
 
@@ -94,24 +94,24 @@ lemma rel_prod_converse: \<open>(rel_prod a b)\<inverse> = rel_prod (a\<inverse>
 lemma rel_prod_Id[simp]: "rel_prod Id Id = Id"
   by (auto simp: rel_prod_def Id_def case_prod_beta image_def)
 
-lemma update_hom_o_2hom_is_2hom: \<open>update_2hom F2 \<Longrightarrow> update_hom G \<Longrightarrow> update_2hom (\<lambda>a b. G (F2 a b))\<close>
-  unfolding update_2hom_def update_hom_def apply auto 
+lemma update_hom_o_2hom_is_2hom: \<open>update_2hom F2 \<Longrightarrow> preregister G \<Longrightarrow> update_2hom (\<lambda>a b. G (F2 a b))\<close>
+  unfolding update_2hom_def preregister_def apply auto 
   apply (rule_tac x=\<open>R2 O R\<close> in exI)
   by auto
-lemma update_2hom_o_hom_left_is_hom: \<open>update_2hom F2 \<Longrightarrow> update_hom G \<Longrightarrow> update_2hom (\<lambda>a b. F2 (G a) b)\<close>
-  unfolding update_2hom_def update_hom_def apply auto 
+lemma update_2hom_o_hom_left_is_hom: \<open>update_2hom F2 \<Longrightarrow> preregister G \<Longrightarrow> update_2hom (\<lambda>a b. F2 (G a) b)\<close>
+  unfolding update_2hom_def preregister_def apply auto 
   apply (rule_tac x=\<open>rel_prod R Id O R2\<close> in exI)
   apply (auto simp: rel_prod_def case_prod_beta)
   apply fastforce by blast
 
 lemma update_2hom_sym: \<open>update_2hom F2 \<Longrightarrow> update_2hom (\<lambda>a b. F2 b a)\<close> 
-  unfolding update_2hom_def update_hom_def apply auto 
+  unfolding update_2hom_def preregister_def apply auto 
   apply (rule_tac x=\<open>(\<lambda>((a,b),c). ((b,a),c)) ` R2\<close> in exI)
   apply (auto simp: case_prod_beta Image_def)
   apply fastforce by blast
 
-lemma update_2hom_left_is_hom: \<open>update_2hom F2 \<Longrightarrow> update_hom (\<lambda>a. F2 a b)\<close>
-  unfolding update_2hom_def update_hom_def apply auto 
+lemma update_2hom_left_is_hom: \<open>update_2hom F2 \<Longrightarrow> preregister (\<lambda>a. F2 a b)\<close>
+  unfolding update_2hom_def preregister_def apply auto 
   apply (rule_tac x=\<open>{(a',c')| a' b' c'. ((a',b'),c') \<in> R2 \<and> b' \<in> b}\<close> in exI)
   by fastforce
 
@@ -130,13 +130,13 @@ lemma tensor_update_is_2hom: \<open>update_2hom tensor_update\<close>
   by force
 
 definition tensor_lift :: \<open>('a, 'b, 'c) update_2hom
-                            \<Rightarrow> (('a\<times>'b, 'c) update_hom)\<close>
+                            \<Rightarrow> (('a\<times>'b, 'c) preregister)\<close>
   where "tensor_lift F2 ab = {(cx,cy)| cx cy ax ay bx by. ((ax,bx),(ay,by)) \<in> ab
              \<and> (((ax,ay), (bx,by)), (cx,cy)) \<in> rel_of_update_2hom F2}"
 
-lemma tensor_lift_hom: 
+lemma tensor_lift_clinear: 
   assumes "update_2hom F2"
-  shows "update_hom (tensor_lift F2)"
+  shows "preregister (tensor_lift F2)"
 proof -
   define R2 where "R2 = rel_of_update_2hom F2"
   from assms
@@ -147,7 +147,7 @@ proof -
    unfolding tensor_lift_def R2_def[symmetric]
    using R_def by blast
   then show ?thesis
-    unfolding update_hom_def by auto
+    unfolding preregister_def by auto
 qed
 
 lemma tensor_lift_correct: 
@@ -180,14 +180,14 @@ proof (intro ext)
 qed
 
 lemma tensor_extensionality:
-  assumes \<open>update_hom F\<close>
-  assumes \<open>update_hom G\<close>
+  assumes \<open>preregister F\<close>
+  assumes \<open>preregister G\<close>
   assumes \<open>\<And>a b. F (tensor_update a b) = G (tensor_update a b)\<close>
   shows "F = G"
 proof -
-  define RF RG where "RF = rel_of_update_hom F" and "RG = rel_of_update_hom G"
+  define RF RG where "RF = rel_of_preregister F" and "RG = rel_of_preregister G"
   then have RF: "F = Image RF" and RG: "G = Image RG"
-    using rel_of_update_hom assms by auto
+    using rel_of_preregister assms by auto
   with assms have RFRG: "RF `` tensor_update a b = RG `` tensor_update a b" for a b
     by auto
   have "RF = RG"
@@ -213,31 +213,31 @@ proof -
     using RF RG by simp
 qed
 
-definition lvalue :: \<open>('a,'b) update_hom \<Rightarrow> bool\<close> where
-  \<open>lvalue F \<longleftrightarrow> update_hom F \<and> (\<forall>a a'. F a O F a' = F (a O a')) \<and> F Id = Id \<and> (\<forall>a. F (a\<inverse>) = (F a)\<inverse>)\<close>
+definition register :: \<open>('a,'b) preregister \<Rightarrow> bool\<close> where
+  \<open>register F \<longleftrightarrow> preregister F \<and> (\<forall>a a'. F a O F a' = F (a O a')) \<and> F Id = Id \<and> (\<forall>a. F (a\<inverse>) = (F a)\<inverse>)\<close>
 
-lemma lvalue_of_id: \<open>lvalue F \<Longrightarrow> F id_update = id_update\<close>
-  by (simp add: lvalue_def)
+lemma register_id: \<open>register F \<Longrightarrow> F id_update = id_update\<close>
+  by (simp add: register_def)
 
-lemma update_hom_tensor_left_is_hom: \<open>update_hom (\<lambda>a. tensor_update a b)\<close>
-  unfolding update_hom_def apply (rule exI[of _ \<open>{((a1,a2),((a1,b1),(a2,b2)))| a1 a2 b1 b2. (b1,b2) \<in> b}\<close>])
+lemma preregister_tensor_left: \<open>preregister (\<lambda>a. tensor_update a b)\<close>
+  unfolding preregister_def apply (rule exI[of _ \<open>{((a1,a2),((a1,b1),(a2,b2)))| a1 a2 b1 b2. (b1,b2) \<in> b}\<close>])
   apply (auto intro!: ext simp: Image_def[abs_def] rel_prod_def case_prod_beta image_def Id_def)
   by (metis fst_conv snd_conv)
-lemma update_hom_tensor_right_is_hom: \<open>update_hom (\<lambda>a. tensor_update b a)\<close>
-  unfolding update_hom_def apply (rule exI[of _ \<open>{((a1,a2),((b1,a1),(b2,a2)))| a1 a2 b1 b2. (b1,b2) \<in> b}\<close>])
+lemma preregister_tensor_right: \<open>preregister (\<lambda>a. tensor_update b a)\<close>
+  unfolding preregister_def apply (rule exI[of _ \<open>{((a1,a2),((b1,a1),(b2,a2)))| a1 a2 b1 b2. (b1,b2) \<in> b}\<close>])
   apply (auto intro!: ext simp: Image_def[abs_def] rel_prod_def case_prod_beta image_def Id_def)
   by (metis fst_conv snd_conv)
 
-lemma lvalue_tensor_left: \<open>lvalue (\<lambda>a. tensor_update a id_update)\<close>
-  apply (simp add: lvalue_def update_hom_tensor_left_is_hom)
+lemma register_tensor_left: \<open>register (\<lambda>a. tensor_update a id_update)\<close>
+  apply (simp add: register_def preregister_tensor_left)
   apply (auto simp: rel_prod_def case_prod_beta relcomp_def relcompp_apply image_def)
   apply (metis fst_conv pair_in_Id_conv prod.exhaust_sel)
   apply (metis IdI fst_conv snd_conv)
   apply (metis IdI fst_conv snd_conv)
   by (metis IdI converse_iff fst_swap snd_conv swap_simp)
 
-lemma lvalue_tensor_right: \<open>lvalue (\<lambda>a. tensor_update id_update a)\<close>
-  apply (simp add: lvalue_def update_hom_tensor_right_is_hom)
+lemma register_tensor_right: \<open>register (\<lambda>a. tensor_update id_update a)\<close>
+  apply (simp add: register_def preregister_tensor_right)
   apply (auto simp: rel_prod_def case_prod_beta relcomp_def relcompp_apply image_def)
   apply blast
   apply (metis IdI fst_conv snd_conv)
@@ -247,80 +247,79 @@ lemma lvalue_tensor_right: \<open>lvalue (\<lambda>a. tensor_update id_update a)
 
 
 lemma
-  lvalue_hom: "lvalue F \<Longrightarrow> update_hom F"
-  by (simp add: lvalue_def) 
+  register_preregister: "register F \<Longrightarrow> preregister F"
+  by (simp add: register_def) 
 
 lemma
-  lvalue_comp: "lvalue F \<Longrightarrow> lvalue G \<Longrightarrow> lvalue (G \<circ> F)"  
-  for F :: "('a,'b) update_hom" and G :: "('b,'c) update_hom"
-  by (simp add: comp_update_hom lvalue_def) 
+  register_comp: "register F \<Longrightarrow> register G \<Longrightarrow> register (G \<circ> F)"  
+  for F :: "('a,'b) preregister" and G :: "('b,'c) preregister"
+  by (simp add: comp_preregister register_def) 
 
 lemma
-  lvalue_mult: "lvalue F \<Longrightarrow> comp_update (F a) (F b) = F (comp_update a b)"
-  by (simp add: lvalue_def)
+  register_mult: "register F \<Longrightarrow> comp_update (F a) (F b) = F (comp_update a b)"
+  by (simp add: register_def)
 
-definition lvalue_pair ::
+definition register_pair ::
   \<open>('a update \<Rightarrow> 'c update) \<Rightarrow> ('b update \<Rightarrow> 'c update) \<Rightarrow> (('a\<times>'b) update \<Rightarrow> 'c update)\<close> where
-  \<open>lvalue_pair F G = tensor_lift (\<lambda>a b. comp_update (F a) (G b))\<close>
+  \<open>register_pair F G = tensor_lift (\<lambda>a b. comp_update (F a) (G b))\<close>
 
-lemma update_2hom_G_O_F: \<open>update_hom F \<Longrightarrow> update_hom G \<Longrightarrow> update_2hom (\<lambda>a b. G b O F a)\<close>
+lemma update_2hom_G_O_F: \<open>preregister F \<Longrightarrow> preregister G \<Longrightarrow> update_2hom (\<lambda>a b. G b O F a)\<close>
   apply (rule update_2hom_o_hom_left_is_hom)
    apply (rule update_2hom_sym)
    apply (rule update_2hom_o_hom_left_is_hom)
     apply (rule update_2hom_sym)
   by (rule comp_update_is_2hom)
 
-lemma lvalue_pair_apply: 
-  assumes [simp]: \<open>lvalue F\<close> \<open>lvalue G\<close>
+lemma register_pair_apply: 
+  assumes [simp]: \<open>register F\<close> \<open>register G\<close>
   assumes \<open>\<And>a b. comp_update (F a) (G b) = comp_update (G b) (F a)\<close>
-  shows \<open>(lvalue_pair F G) (tensor_update a b) = comp_update (F a) (G b)\<close>
-  unfolding lvalue_pair_def
+  shows \<open>(register_pair F G) (tensor_update a b) = comp_update (F a) (G b)\<close>
+  unfolding register_pair_def
   apply (subst tensor_lift_correct[THEN fun_cong, THEN fun_cong])
    apply (rule update_2hom_G_O_F)
-  by (simp_all add: lvalue_hom)
+  by (simp_all add: register_preregister)
 
-lemma lvalue_pair_lvalue:
+lemma register_pair_is_register:
   fixes F :: \<open>'a update \<Rightarrow> 'c update\<close> and G
-  assumes [simp]: \<open>lvalue F\<close> and [simp]: \<open>lvalue G\<close>
+  assumes [simp]: \<open>register F\<close> and [simp]: \<open>register G\<close>
   assumes compat: \<open>\<And>a b. comp_update (F a) (G b) = comp_update (G b) (F a)\<close>
-  shows \<open>lvalue (lvalue_pair F G)\<close> 
-  (* assumes ptensor: \<open>\<And>a b. p (tensor_update a b) = comp_update (F a) (G b)\<close> *)
-proof (unfold lvalue_def, intro conjI allI)
-  define p where \<open>p = (lvalue_pair F G)\<close>
-  show [simp]: \<open>update_hom p\<close>
-    unfolding p_def lvalue_pair_def 
-    apply (rule tensor_lift_hom)
+  shows \<open>register (register_pair F G)\<close> 
+proof (unfold register_def, intro conjI allI)
+  define p where \<open>p = (register_pair F G)\<close>
+  show [simp]: \<open>preregister p\<close>
+    unfolding p_def register_pair_def 
+    apply (rule tensor_lift_clinear)
     apply (rule update_2hom_G_O_F)
-    by (simp_all add: lvalue_hom)
+    by (simp_all add: register_preregister)
   have ptensor: \<open>\<And>a b. p (tensor_update a b) = comp_update (F a) (G b)\<close>
-    unfolding p_def lvalue_pair_def apply (subst tensor_lift_correct[THEN fun_cong, THEN fun_cong])
+    unfolding p_def register_pair_def apply (subst tensor_lift_correct[THEN fun_cong, THEN fun_cong])
     apply (rule update_2hom_G_O_F)
-    by (simp_all add: lvalue_hom)
-  have h1: \<open>update_hom (\<lambda>a. p a O p a')\<close> for a'
+    by (simp_all add: register_preregister)
+  have h1: \<open>preregister (\<lambda>a. p a O p a')\<close> for a'
     apply (rule update_2hom_left_is_hom)
     apply (rule update_2hom_o_hom_left_is_hom)
     using comp_update_is_2hom update_2hom_sym by auto
-  have h2: \<open>update_hom (\<lambda>a. p (a O a'))\<close> for a'
+  have h2: \<open>preregister (\<lambda>a. p (a O a'))\<close> for a'
     apply (rule update_2hom_left_is_hom)
     apply (rule update_hom_o_2hom_is_2hom[where G=p])
     using comp_update_is_2hom update_2hom_sym by auto
-  have h3: \<open>update_hom (\<lambda>a'. p a O p a')\<close> for a
+  have h3: \<open>preregister (\<lambda>a'. p a O p a')\<close> for a
     apply (rule update_2hom_left_is_hom)
     apply (rule update_2hom_o_hom_left_is_hom)
     using comp_update_is_2hom update_2hom_sym by auto
-  have h4: \<open>update_hom (\<lambda>a'. p (a O a'))\<close> for a
+  have h4: \<open>preregister (\<lambda>a'. p (a O a'))\<close> for a
     apply (rule update_2hom_left_is_hom)
     apply (rule update_hom_o_2hom_is_2hom[where G=p])
     using comp_update_is_2hom update_2hom_sym by auto
-  have h5: \<open>update_hom (\<lambda>a. p (a\<inverse>))\<close>
-    apply (rule comp_update_hom[where G=p, unfolded o_def])
-    by (simp_all add: converse_hom)
-  have h6: \<open>update_hom (\<lambda>a. (p a)\<inverse>)\<close>
-    apply (rule comp_update_hom[where F=p, unfolded o_def])
-    by (simp_all add: converse_hom)
+  have h5: \<open>preregister (\<lambda>a. p (a\<inverse>))\<close>
+    apply (rule comp_preregister[where G=p, unfolded o_def])
+    by (simp_all add: converse_preregister)
+  have h6: \<open>preregister (\<lambda>a. (p a)\<inverse>)\<close>
+    apply (rule comp_preregister[where F=p, unfolded o_def])
+    by (simp_all add: converse_preregister)
   have \<open>p (tensor_update a1 a2) O p (tensor_update a1' a2') = p ((tensor_update a1 a2) O (tensor_update a1' a2'))\<close> for a1 a2 a1' a2'
     unfolding ptensor tensor_update_mult
-    by (metis assms(1) assms(2) comp_update_assoc lvalue_mult compat) 
+    by (metis assms(1) assms(2) comp_update_assoc register_mult compat) 
   
   then have \<open>p (tensor_update a1 a2) O p a' = p ((tensor_update a1 a2) O a')\<close> for a1 a2 a'
     by (rule tensor_extensionality[OF h3 h4, THEN fun_cong])
@@ -329,12 +328,12 @@ proof (unfold lvalue_def, intro conjI allI)
 
   show \<open>p Id = Id\<close>
     apply (simp flip: rel_prod_Id add: ptensor)
-    by (metis R_O_Id assms(1) assms(2) lvalue_def)
+    by (metis R_O_Id assms(1) assms(2) register_def)
   
   have \<open>p ((tensor_update a1 a2)\<inverse>) = (p (tensor_update a1 a2))\<inverse>\<close> for a1 a2
     apply (simp add: ptensor converse_relcomp rel_prod_converse)
     apply (subst compat)
-    by (metis assms(1) assms(2) lvalue_def)
+    by (metis assms(1) assms(2) register_def)
 
   then show \<open>p (a\<inverse>) = (p a)\<inverse>\<close> for a
     by (rule tensor_extensionality[OF h5 h6, THEN fun_cong])
