Axioms_Quantum.thy
@@ -1,4 +1,4 @@
-section \<open>Quantum instantiation of lvalues\<close>
+section \<open>Quantum instantiation of registers\<close>
 
 (* AXIOM INSTANTIATION (use instantiate_laws.py to generate Laws_Quantum.thy)
 
@@ -8,21 +8,21 @@ section \<open>Quantum instantiation of lvalues\<close>
     # Constants
     comp_update \<rightarrow> timesOp
     id_update \<rightarrow> idOp
-    update_hom \<rightarrow> clinear
+    preregister \<rightarrow> clinear
     tensor_update \<rightarrow> tensor_op
     
     # Lemmas
     id_update_left \<rightarrow> times_idOp2
     id_update_right \<rightarrow> times_idOp1
     comp_update_assoc \<rightarrow> cblinfun_apply_assoc
-    id_update_hom \<rightarrow> complex_vector.linear_id
-    comp_update_hom \<rightarrow> clinear_compose
+    id_preregister \<rightarrow> complex_vector.linear_id
+    comp_preregister \<rightarrow> clinear_compose
     tensor_update_mult \<rightarrow> comp_tensor_op
-    update_hom_tensor_left_is_hom \<rightarrow> clinear_tensor_right
-    update_hom_tensor_right_is_hom \<rightarrow> clinear_tensor_left
+    preregister_tensor_left \<rightarrow> clinear_tensor_right
+    preregister_tensor_right \<rightarrow> clinear_tensor_left
 
     # Chapter name
-    Generic laws about lvalues \<rightarrow> Generic laws about lvalues, instantiated quantumly
+    Generic laws about registers \<rightarrow> Generic laws about registers, instantiated quantumly
 *)
 
 theory Axioms_Quantum
@@ -37,184 +37,113 @@ no_notation m_inv ("inv\<index> _" [81] 80)
 
 type_synonym 'a update = \<open>('a ell2, 'a ell2) cblinfun\<close>
 
-(* lemma update_hom_o_2hom_is_2hom: \<open>cbilinear F2 \<Longrightarrow> clinear G \<Longrightarrow> cbilinear (\<lambda>a b. G (F2 a b))\<close>
-  apply (auto simp: cbilinear_def intro!: clinearI)
-  apply (smt (z3) clinear_additive_D)
-  apply (metis complex_vector.linear_scale)
-   apply (simp add: clinear_additive_D)
-  by (simp add: complex_vector.linear_scale)
-lemma update_2hom_o_hom_left_is_hom: \<open>cbilinear F2 \<Longrightarrow> clinear G \<Longrightarrow> cbilinear (\<lambda>a b. F2 (G a) b)\<close>
-  apply (auto simp: cbilinear_def intro!: clinearI)
-  apply (smt (z3) clinear_additive_D)
-  by (metis (full_types) complex_vector.linear_scale)
-lemma update_2hom_sym: \<open>cbilinear F2 \<Longrightarrow> cbilinear (\<lambda>a b. F2 b a)\<close> 
-  by (auto simp: cbilinear_def)
-lemma update_2hom_left_is_hom: \<open>cbilinear F2 \<Longrightarrow> clinear (\<lambda>a. F2 a b)\<close>
-  by (auto simp: cbilinear_def) *)
-
-lemma update_hom_mult_right: \<open>clinear (\<lambda>a. a o\<^sub>C\<^sub>L z)\<close>
+lemma preregister_mult_right: \<open>clinear (\<lambda>a. a o\<^sub>C\<^sub>L z)\<close>
   by (simp add: cblinfun_apply_dist1 clinearI)
-lemma update_hom_mult_left: \<open>clinear (\<lambda>a. z o\<^sub>C\<^sub>L a)\<close>
+lemma preregister_mult_left: \<open>clinear (\<lambda>a. z o\<^sub>C\<^sub>L a)\<close>
   by (simp add: cblinfun_apply_dist2 clinearI)
 
-definition lvalue :: \<open>('a::finite update \<Rightarrow> 'b::finite update) \<Rightarrow> bool\<close> where
-  "lvalue F \<longleftrightarrow> 
+definition register :: \<open>('a::finite update \<Rightarrow> 'b::finite update) \<Rightarrow> bool\<close> where
+  "register F \<longleftrightarrow> 
      clinear F
    \<and> F idOp = idOp 
    \<and> (\<forall>a b. F(a o\<^sub>C\<^sub>L b) = F a o\<^sub>C\<^sub>L F b)
    \<and> (\<forall>a. F (a*) = (F a)*)"
 
-lemma lvalue_of_id: \<open>lvalue F \<Longrightarrow> F idOp = idOp\<close>
-  by (simp add: lvalue_def)
+lemma register_id: \<open>register F \<Longrightarrow> F idOp = idOp\<close>
+  by (simp add: register_def)
 
-lemma lvalue_hom: "lvalue F \<Longrightarrow> clinear F"
-  unfolding lvalue_def by simp
+lemma register_preregister: "register F \<Longrightarrow> clinear F"
+  unfolding register_def by simp
 
-lemma lvalue_comp: "lvalue F \<Longrightarrow> lvalue G \<Longrightarrow> lvalue (G \<circ> F)"
-  unfolding lvalue_def
+lemma register_comp: "register F \<Longrightarrow> register G \<Longrightarrow> register (G \<circ> F)"
+  unfolding register_def
   apply auto
   using clinear_compose by blast
 
-lemma lvalue_mult: "lvalue F \<Longrightarrow> timesOp (F a) (F b) = F (timesOp a b)"
-  unfolding lvalue_def
+lemma register_mult: "register F \<Longrightarrow> timesOp (F a) (F b) = F (timesOp a b)"
+  unfolding register_def
   by auto
 
-lemma lvalue_tensor_left: \<open>lvalue (\<lambda>a. tensor_op a idOp)\<close>
-  by (simp add: comp_tensor_op lvalue_def tensor_op_cbilinear tensor_op_adjoint)
+lemma register_tensor_left: \<open>register (\<lambda>a. tensor_op a idOp)\<close>
+  by (simp add: comp_tensor_op register_def tensor_op_cbilinear tensor_op_adjoint)
 
-lemma lvalue_tensor_right: \<open>lvalue (\<lambda>a. tensor_op idOp a)\<close>
-  by (simp add: comp_tensor_op lvalue_def tensor_op_cbilinear tensor_op_adjoint)
+lemma register_tensor_right: \<open>register (\<lambda>a. tensor_op idOp a)\<close>
+  by (simp add: comp_tensor_op register_def tensor_op_cbilinear tensor_op_adjoint)
 
 
-definition lvalue_pair ::
+definition register_pair ::
   \<open>('a::finite update \<Rightarrow> 'c::finite update) \<Rightarrow> ('b::finite update \<Rightarrow> 'c update)
          \<Rightarrow> (('a\<times>'b) update \<Rightarrow> 'c update)\<close> where
-  \<open>lvalue_pair F G = tensor_lift (\<lambda>a b. F a o\<^sub>C\<^sub>L G b)\<close>
+  \<open>register_pair F G = tensor_lift (\<lambda>a b. F a o\<^sub>C\<^sub>L G b)\<close>
 
 lemma cbilinear_F_comp_G[simp]: \<open>clinear F \<Longrightarrow> clinear G \<Longrightarrow> cbilinear (\<lambda>a b. F a o\<^sub>C\<^sub>L G b)\<close>
   unfolding cbilinear_def
   by (auto simp add: clinear_iff cblinfun_apply_dist1 cblinfun_apply_dist2)
 
-lemma lvalue_pair_apply: 
-  assumes \<open>lvalue F\<close> and \<open>lvalue G\<close>
+lemma register_pair_apply: 
+  assumes \<open>register F\<close> and \<open>register G\<close>
   assumes \<open>\<And>a b. F a o\<^sub>C\<^sub>L G b = G b o\<^sub>C\<^sub>L F a\<close>
-  shows \<open>(lvalue_pair F G) (tensor_op a b) = F a o\<^sub>C\<^sub>L G b\<close>
-  unfolding lvalue_pair_def
+  shows \<open>(register_pair F G) (tensor_op a b) = F a o\<^sub>C\<^sub>L G b\<close>
+  unfolding register_pair_def
   apply (subst tensor_lift_correct[THEN fun_cong, THEN fun_cong])
   apply (rule cbilinear_F_comp_G)
   using assms apply (auto intro!: cbilinear_F_comp_G)
-  using lvalue_def by auto
+  using register_def by auto
 
-lemma lvalue_pair_lvalue:
+lemma register_pair_is_register:
   fixes F :: \<open>'a::finite update \<Rightarrow> 'c::finite update\<close> and G
-  assumes [simp]: \<open>lvalue F\<close> and [simp]: \<open>lvalue G\<close>
+  assumes [simp]: \<open>register F\<close> and [simp]: \<open>register G\<close>
   assumes \<open>\<And>a b. F a o\<^sub>C\<^sub>L G b = G b o\<^sub>C\<^sub>L F a\<close>
-  shows \<open>lvalue (lvalue_pair F G)\<close> 
-proof (unfold lvalue_def, intro conjI allI)
+  shows \<open>register (register_pair F G)\<close> 
+proof (unfold register_def, intro conjI allI)
   have [simp]: \<open>clinear F\<close> \<open>clinear G\<close>
-    using assms lvalue_def by blast+
+    using assms register_def by blast+
   have [simp]: \<open>F idOp = idOp\<close> \<open>G idOp = idOp\<close>
-    using assms(1,2) lvalue_def by blast+
-  show [simp]: \<open>clinear (lvalue_pair F G)\<close>
-    unfolding lvalue_pair_def apply (rule tensor_lift_hom)
+    using assms(1,2) register_def by blast+
+  show [simp]: \<open>clinear (register_pair F G)\<close>
+    unfolding register_pair_def apply (rule tensor_lift_clinear)
     by simp
-  show \<open>lvalue_pair F G idOp = idOp\<close>
+  show \<open>register_pair F G idOp = idOp\<close>
     apply (simp flip: tensor_id)
-    apply (subst lvalue_pair_apply)
+    apply (subst register_pair_apply)
     using assms by simp_all
-  have [simp]: \<open>clinear (\<lambda>y. lvalue_pair F G (x o\<^sub>C\<^sub>L y))\<close> for x :: \<open>('a\<times>'b) update\<close>
-    apply (rule clinear_compose[unfolded o_def, where g=\<open>lvalue_pair F G\<close>])
+  have [simp]: \<open>clinear (\<lambda>y. register_pair F G (x o\<^sub>C\<^sub>L y))\<close> for x :: \<open>('a\<times>'b) update\<close>
+    apply (rule clinear_compose[unfolded o_def, where g=\<open>register_pair F G\<close>])
     by (simp_all add: cblinfun_apply_dist2 clinearI)
-  have [simp]: \<open>clinear (\<lambda>y. x o\<^sub>C\<^sub>L lvalue_pair F G y)\<close> for x :: \<open>'c update\<close>
-    apply (rule clinear_compose[unfolded o_def, where f=\<open>lvalue_pair F G\<close>])
+  have [simp]: \<open>clinear (\<lambda>y. x o\<^sub>C\<^sub>L register_pair F G y)\<close> for x :: \<open>'c update\<close>
+    apply (rule clinear_compose[unfolded o_def, where f=\<open>register_pair F G\<close>])
     by (simp_all add: cblinfun_apply_dist2 clinearI)
-  have [simp]: \<open>clinear (\<lambda>x. lvalue_pair F G (x o\<^sub>C\<^sub>L y))\<close> for y :: \<open>('a\<times>'b) update\<close>
-    apply (rule clinear_compose[unfolded o_def, where g=\<open>lvalue_pair F G\<close>])
+  have [simp]: \<open>clinear (\<lambda>x. register_pair F G (x o\<^sub>C\<^sub>L y))\<close> for y :: \<open>('a\<times>'b) update\<close>
+    apply (rule clinear_compose[unfolded o_def, where g=\<open>register_pair F G\<close>])
     by (simp_all add: cblinfun_apply_dist1 clinearI)
-  have [simp]: \<open>clinear (\<lambda>x. lvalue_pair F G x o\<^sub>C\<^sub>L y)\<close> for y :: \<open>'c update\<close>
-    apply (rule clinear_compose[unfolded o_def, where f=\<open>lvalue_pair F G\<close>])
+  have [simp]: \<open>clinear (\<lambda>x. register_pair F G x o\<^sub>C\<^sub>L y)\<close> for y :: \<open>'c update\<close>
+    apply (rule clinear_compose[unfolded o_def, where f=\<open>register_pair F G\<close>])
     by (simp_all add: cblinfun_apply_dist1 clinearI)
   have [simp]: \<open>F (x o\<^sub>C\<^sub>L y) = F x o\<^sub>C\<^sub>L F y\<close> for x y
-    by (simp add: lvalue_mult)
+    by (simp add: register_mult)
   have [simp]: \<open>G (x o\<^sub>C\<^sub>L y) = G x o\<^sub>C\<^sub>L G y\<close> for x y
-    by (simp add: lvalue_mult)
-  have [simp]: \<open>clinear (\<lambda>a. (lvalue_pair F G (a*))*)\<close>
+    by (simp add: register_mult)
+  have [simp]: \<open>clinear (\<lambda>a. (register_pair F G (a*))*)\<close>
     apply (rule antilinear_o_antilinear[unfolded o_def, where f=\<open>adj\<close>])
      apply (simp add: Adj_cblinfun_plus antilinearI)
     apply (rule antilinear_o_clinear[unfolded o_def, where g=\<open>adj\<close>])
     by (simp_all add: Adj_cblinfun_plus antilinearI)
   have [simp]: \<open>F (a*) = (F a)*\<close> for a
-    using assms(1) lvalue_def by blast
+    using assms(1) register_def by blast
   have [simp]: \<open>G (b*) = (G b)*\<close> for b
-    using assms(2) lvalue_def by blast
+    using assms(2) register_def by blast
 
   fix a b
-  show \<open>lvalue_pair F G (a o\<^sub>C\<^sub>L b) = lvalue_pair F G a o\<^sub>C\<^sub>L lvalue_pair F G b\<close>
+  show \<open>register_pair F G (a o\<^sub>C\<^sub>L b) = register_pair F G a o\<^sub>C\<^sub>L register_pair F G b\<close>
     apply (rule tensor_extensionality[THEN fun_cong, where x=b], simp_all)
     apply (rule tensor_extensionality[THEN fun_cong, where x=a], simp_all)
-    apply (simp_all add: comp_tensor_op lvalue_pair_apply assms(3))
+    apply (simp_all add: comp_tensor_op register_pair_apply assms(3))
     using assms(3) by (metis assoc_left(1)) 
-  have \<open>(lvalue_pair F G (a*))* = lvalue_pair F G a\<close>
+  have \<open>(register_pair F G (a*))* = register_pair F G a\<close>
     apply (rule tensor_extensionality[THEN fun_cong, where x=a])
-    by (simp_all add: tensor_op_adjoint lvalue_pair_apply assms(3))
-  then show \<open>lvalue_pair F G (a*) = lvalue_pair F G a*\<close>
+    by (simp_all add: tensor_op_adjoint register_pair_apply assms(3))
+  then show \<open>register_pair F G (a*) = register_pair F G a*\<close>
     by (metis adjoint_twice)
 qed
-
-
-(* lemma pair_lvalue_axiom: 
-  fixes F :: \<open>'a::finite update \<Rightarrow> 'c::finite update\<close> and G :: \<open>'b::finite update \<Rightarrow> 'c update\<close>
-  assumes \<open>lvalue F\<close> and \<open>lvalue G\<close> and [simp]: \<open>clinear p\<close>
-  assumes compat: \<open>\<And>a b. F a o\<^sub>C\<^sub>L G b = G b o\<^sub>C\<^sub>L F a\<close>
-  assumes tensor: \<open>\<And>a b. p (tensor_op a b) = F a o\<^sub>C\<^sub>L G b\<close>
-  shows \<open>lvalue p\<close>
-proof (unfold lvalue_def, intro conjI allI)
-  have h1: \<open>clinear (\<lambda>a. p (a o\<^sub>C\<^sub>L b))\<close> for b :: "('a \<times> 'b) update"
-    apply (rule linear_compose[unfolded o_def, of _ p])
-     apply (simp add: cblinfun_apply_dist1 clinearI)
-    by simp
-  have h2: \<open>clinear (\<lambda>a. p a o\<^sub>C\<^sub>L p b)\<close> for b
-    apply (rule linear_compose[unfolded o_def, of p])
-    apply simp
-    by (meson cblinfun_apply_dist1 clinearI scalar_op_op)
-  have h3: \<open>clinear (\<lambda>c. p (d o\<^sub>C\<^sub>L c))\<close> for d :: "('a \<times> 'b) update"
-    apply (rule linear_compose[unfolded o_def, of _ p])
-     apply (simp add: cblinfun_apply_dist2 clinearI)
-    by simp
-  have h4: \<open>clinear (\<lambda>c. p d o\<^sub>C\<^sub>L p c)\<close> for d
-    apply (rule linear_compose[unfolded o_def, of p])
-    apply simp
-    by (simp add: cblinfun_apply_dist2 clinearI)
-
-  fix x y :: \<open>('a \<times> 'b) ell2 \<Rightarrow>\<^sub>C\<^sub>L ('a \<times> 'b) ell2\<close>
-  show "clinear p"
-    using assms by auto
-  show \<open>p idOp = idOp\<close>
-    unfolding tensor_id[symmetric] tensor
-    using \<open>lvalue F\<close> \<open>lvalue G\<close> unfolding lvalue_def by auto
-
-  have *: \<open>p (tensor_op a b o\<^sub>C\<^sub>L tensor_op a' b') = p (tensor_op a b) o\<^sub>C\<^sub>L p (tensor_op a' b')\<close> for a b a' b'
-    using \<open>lvalue F\<close> \<open>lvalue G\<close>
-    apply (simp add: tensor comp_tensor_op lvalue_def)
-    by (metis cblinfun_apply_assoc compat)
-  show \<open>p (x o\<^sub>C\<^sub>L y) = p x o\<^sub>C\<^sub>L p y\<close>
-    using h1 h2 apply (rule tensor_extensionality[THEN fun_cong, where x=x])
-    using h3 h4 apply (rule tensor_extensionality[THEN fun_cong, where x=y])
-    using * by -
-
-  have hom_padjadj: \<open>clinear (\<lambda>a. p (a* )* )\<close>
-    using \<open>clinear p\<close>
-    by (auto simp: Adj_cblinfun_plus complex_vector.linear_add complex_vector.linear_scale intro!: clinearI)
-
-  have *: \<open>(p (tensor_op a b* ))* = p (tensor_op a b)\<close> for a b
-    using \<open>lvalue F\<close> \<open>lvalue G\<close>
-    by (simp add: compat tensor tensor_op_adjoint lvalue_def)
-  have \<open>(p (x* ))* = p x\<close>
-    apply (rule fun_cong[where x=x])
-    apply (rule tensor_extensionality)
-    using hom_padjadj * by simp_all
-  then show \<open>p (x* ) = (p x)*\<close>
-    by (metis adjoint_twice)
-qed *)
 
 end
