Laws.thy
@@ -1,4 +1,4 @@
-section \<open>Generic laws about lvalues\<close>
+section \<open>Generic laws about registers\<close>
 
 theory Laws
   imports Axioms "HOL-Library.Rewrite" Misc
@@ -9,147 +9,146 @@ no_notation Group.mult (infixl "\<otimes>\<index>" 70)
 text \<open>This notation is only used inside this file\<close>
 notation comp_update (infixl "*\<^sub>u" 55)
 notation tensor_update (infixr "\<otimes>\<^sub>u" 70)
-notation lvalue_pair ("'(_;_')")
+notation register_pair ("'(_;_')")
 
 subsection \<open>Elementary facts\<close>
 
-declare id_update_hom[simp]
+declare id_preregister[simp]
 declare id_update_left[simp]
 declare id_update_right[simp]
-declare lvalue_hom[simp]
-declare lvalue_comp[simp]
-declare lvalue_of_id[simp]
-declare lvalue_tensor_left[simp]
-declare lvalue_tensor_right[simp]
-declare update_hom_mult_right[simp]
-declare update_hom_mult_left[simp]
-declare update_hom_tensor_left_is_hom[simp]
-declare update_hom_tensor_right_is_hom[simp]
+declare register_preregister[simp]
+declare register_comp[simp]
+declare register_id[simp]
+declare register_tensor_left[simp]
+declare register_tensor_right[simp]
+declare preregister_mult_right[simp]
+declare preregister_mult_left[simp]
+declare preregister_tensor_left[simp]
+declare preregister_tensor_right[simp]
 
 
 subsection \<open>Lvalues\<close>
 
-lemma id_update_tensor_lvalue[simp]:
-  assumes \<open>lvalue F\<close>
-  shows \<open>lvalue (\<lambda>a::'a::domain update. id_update \<otimes>\<^sub>u F a)\<close>
-  using assms apply (rule lvalue_comp[unfolded o_def])
+lemma id_update_tensor_register[simp]:
+  assumes \<open>register F\<close>
+  shows \<open>register (\<lambda>a::'a::domain update. id_update \<otimes>\<^sub>u F a)\<close>
+  using assms apply (rule register_comp[unfolded o_def])
   by simp
 
-lemma lvalue_tensor_id_update[simp]:
-  assumes \<open>lvalue F\<close>
-  shows \<open>lvalue (\<lambda>a::'a::domain update. F a \<otimes>\<^sub>u id_update)\<close>
-  using assms apply (rule lvalue_comp[unfolded o_def])
-  by (simp add: lvalue_tensor_left)
+lemma register_tensor_id_update[simp]:
+  assumes \<open>register F\<close>
+  shows \<open>register (\<lambda>a::'a::domain update. F a \<otimes>\<^sub>u id_update)\<close>
+  using assms apply (rule register_comp[unfolded o_def])
+  by simp
 
 subsection \<open>Tensor product of homs\<close>
 
-(* TODO: rename \<rightarrow> lvalue_tensor *)
-definition tensor_update_hom  (infixr "\<otimes>\<^sub>h" 70) where
-  "tensor_update_hom F G = lvalue_pair (\<lambda>a. tensor_update (F a) id_update) (\<lambda>b. tensor_update id_update (G b))"
+definition register_tensor  (infixr "\<otimes>\<^sub>h" 70) where
+  "register_tensor F G = register_pair (\<lambda>a. tensor_update (F a) id_update) (\<lambda>b. tensor_update id_update (G b))"
 
-lemma tensor_update_hom_is_hom: 
+lemma register_tensor_is_hom: 
   fixes F :: "'a::domain update \<Rightarrow> 'b::domain update" and G :: "'c::domain update \<Rightarrow> 'd::domain update"
-  shows "lvalue F \<Longrightarrow> lvalue G \<Longrightarrow> lvalue (F \<otimes>\<^sub>h G)"
-  unfolding tensor_update_hom_def
-  apply (rule lvalue_pair_lvalue)
+  shows "register F \<Longrightarrow> register G \<Longrightarrow> register (F \<otimes>\<^sub>h G)"
+  unfolding register_tensor_def
+  apply (rule register_pair_is_register)
   by (simp_all add: tensor_update_mult)
 
-lemma tensor_update_hom_apply[simp]:
+lemma register_tensor_apply[simp]:
   fixes F :: "'a::domain update \<Rightarrow> 'b::domain update" and G :: "'c::domain update \<Rightarrow> 'd::domain update"
-  assumes \<open>lvalue F\<close> and \<open>lvalue G\<close>
+  assumes \<open>register F\<close> and \<open>register G\<close>
   shows "(F \<otimes>\<^sub>h G) (a \<otimes>\<^sub>u b) = F a \<otimes>\<^sub>u G b"
-  unfolding tensor_update_hom_def
-  apply (subst lvalue_pair_apply)
-  unfolding tensor_update_hom_def 
+  unfolding register_tensor_def
+  apply (subst register_pair_apply)
+  unfolding register_tensor_def 
   by (simp_all add: assms tensor_update_mult)
 
-definition "update_basis (_::'b::domain itself) A \<longleftrightarrow> 
-  (\<forall>F G :: 'a::domain update \<Rightarrow> 'b update. update_hom F \<longrightarrow> update_hom G \<longrightarrow> (\<forall>x\<in>A. F x = G x) \<longrightarrow> F = G)"
+definition "update_base (_::'b::domain itself) A \<longleftrightarrow> 
+  (\<forall>F G :: 'a::domain update \<Rightarrow> 'b update. preregister F \<longrightarrow> preregister G \<longrightarrow> (\<forall>x\<in>A. F x = G x) \<longrightarrow> F = G)"
 
-lemma update_basis_UNIV[simp]: \<open>update_basis TYPE(_) UNIV\<close>
-  unfolding update_basis_def by auto
+lemma update_base_UNIV[simp]: \<open>update_base TYPE(_) UNIV\<close>
+  unfolding update_base_def by auto
 
-lemma update_basis_mono: \<open>A \<subseteq> B \<Longrightarrow> update_basis TYPE('a::domain) A \<Longrightarrow> update_basis TYPE('a) B\<close>
-  unfolding update_basis_def by (meson in_mono) 
+lemma update_base_mono: \<open>A \<subseteq> B \<Longrightarrow> update_base TYPE('a::domain) A \<Longrightarrow> update_base TYPE('a) B\<close>
+  unfolding update_base_def by (meson in_mono) 
 
-lemma lvalue_eqI: \<open>update_basis TYPE('b::domain) A \<Longrightarrow> update_hom F \<Longrightarrow> update_hom G \<Longrightarrow> (\<And>x. x\<in>A \<Longrightarrow> F x = G x) \<Longrightarrow> F = (G::_ \<Rightarrow> 'b update)\<close>
-  unfolding update_basis_def by auto
+lemma register_eqI: \<open>update_base TYPE('b::domain) A \<Longrightarrow> preregister F \<Longrightarrow> preregister G \<Longrightarrow> (\<And>x. x\<in>A \<Longrightarrow> F x = G x) \<Longrightarrow> F = (G::_ \<Rightarrow> 'b update)\<close>
+  unfolding update_base_def by auto
 
-lemma update_basis_tensor:
+lemma update_base_tensor:
   fixes A :: \<open>'a::domain update set\<close> and B :: \<open>'b::domain update set\<close>
-  assumes [simp]: \<open>update_basis TYPE('c::domain) A\<close>
-  assumes [simp]: \<open>update_basis TYPE('c) B\<close>
-  shows \<open>update_basis TYPE('c) {a \<otimes>\<^sub>u b | a b. a\<in>A \<and> b\<in>B}\<close>
-proof (unfold update_basis_def, intro allI impI)
+  assumes [simp]: \<open>update_base TYPE('c::domain) A\<close>
+  assumes [simp]: \<open>update_base TYPE('c) B\<close>
+  shows \<open>update_base TYPE('c) {a \<otimes>\<^sub>u b | a b. a\<in>A \<and> b\<in>B}\<close>
+proof (unfold update_base_def, intro allI impI)
   fix F G :: \<open>('a\<times>'b) update \<Rightarrow> 'c update\<close>
-  assume [simp]: \<open>update_hom F\<close> \<open>update_hom G\<close>
-  have [simp]: \<open>update_hom (\<lambda>x. F (a \<otimes>\<^sub>u x))\<close> for a
-    using _ \<open>update_hom F\<close> apply (rule comp_update_hom[unfolded o_def])
+  assume [simp]: \<open>preregister F\<close> \<open>preregister G\<close>
+  have [simp]: \<open>preregister (\<lambda>x. F (a \<otimes>\<^sub>u x))\<close> for a
+    using _ \<open>preregister F\<close> apply (rule comp_preregister[unfolded o_def])
     by simp
-  have [simp]: \<open>update_hom (\<lambda>x. G (a \<otimes>\<^sub>u x))\<close> for a
-    using _ \<open>update_hom G\<close> apply (rule comp_update_hom[unfolded o_def])
+  have [simp]: \<open>preregister (\<lambda>x. G (a \<otimes>\<^sub>u x))\<close> for a
+    using _ \<open>preregister G\<close> apply (rule comp_preregister[unfolded o_def])
     by simp
-  have [simp]: \<open>update_hom (\<lambda>x. F (x \<otimes>\<^sub>u b))\<close> for b
-    using _ \<open>update_hom F\<close> apply (rule comp_update_hom[unfolded o_def])
+  have [simp]: \<open>preregister (\<lambda>x. F (x \<otimes>\<^sub>u b))\<close> for b
+    using _ \<open>preregister F\<close> apply (rule comp_preregister[unfolded o_def])
     by simp
-  have [simp]: \<open>update_hom (\<lambda>x. G (x \<otimes>\<^sub>u b))\<close> for b
-    using _ \<open>update_hom G\<close> apply (rule comp_update_hom[unfolded o_def])
+  have [simp]: \<open>preregister (\<lambda>x. G (x \<otimes>\<^sub>u b))\<close> for b
+    using _ \<open>preregister G\<close> apply (rule comp_preregister[unfolded o_def])
     by simp
 
   assume \<open>\<forall>x\<in>{a \<otimes>\<^sub>u b |a b. a\<in>A \<and> b\<in>B}. F x = G x\<close>
   then have EQ: \<open>F (a \<otimes>\<^sub>u b) = G (a \<otimes>\<^sub>u b)\<close> if \<open>a \<in> A\<close> and \<open>b \<in> B\<close> for a b
     using that by auto
   then have \<open>F (a \<otimes>\<^sub>u b) = G (a \<otimes>\<^sub>u b)\<close> if \<open>a \<in> A\<close> for a b
-    apply (rule lvalue_eqI[where A=B, THEN fun_cong, where x=b, rotated -1])
+    apply (rule register_eqI[where A=B, THEN fun_cong, where x=b, rotated -1])
     using that by auto
   then have \<open>F (a \<otimes>\<^sub>u b) = G (a \<otimes>\<^sub>u b)\<close> for a b
-    apply (rule lvalue_eqI[where A=A, THEN fun_cong, where x=a, rotated -1])
+    apply (rule register_eqI[where A=A, THEN fun_cong, where x=a, rotated -1])
     by auto
   then show "F = G"
     apply (rule tensor_extensionality[rotated -1])
     by auto
 qed
 
-(* Easier to apply using 'rule' than update_basis_tensor *)
-lemma update_basis_tensor':
+(* Easier to apply using 'rule' than update_base_tensor *)
+lemma update_base_tensor':
   fixes A :: \<open>'a::domain update set\<close> and B :: \<open>'b::domain update set\<close>
-  assumes \<open>update_basis TYPE('c::domain) A\<close>
-  assumes \<open>update_basis TYPE('c) B\<close>
+  assumes \<open>update_base TYPE('c::domain) A\<close>
+  assumes \<open>update_base TYPE('c) B\<close>
   assumes \<open>C = {a \<otimes>\<^sub>u b | a b. a\<in>A \<and> b\<in>B}\<close>
-  shows \<open>update_basis TYPE('c) C\<close>
+  shows \<open>update_base TYPE('c) C\<close>
   using assms
-  by (simp add: update_basis_tensor)
+  by (simp add: update_base_tensor)
 
 lemma tensor_extensionality3: 
   fixes F G :: \<open>('a::domain\<times>'b::domain\<times>'c::domain) update \<Rightarrow> 'd::domain update\<close>
-  assumes [simp]: \<open>lvalue F\<close> \<open>lvalue G\<close>
+  assumes [simp]: \<open>register F\<close> \<open>register G\<close>
   assumes "\<And>f g h. F (f \<otimes>\<^sub>u g \<otimes>\<^sub>u h) = G (f \<otimes>\<^sub>u g \<otimes>\<^sub>u h)"
   shows "F = G"
-proof (rule lvalue_eqI[where A=\<open>{a\<otimes>\<^sub>ub\<otimes>\<^sub>uc| a b c. True}\<close>])
-  have \<open>update_basis TYPE('d) {b \<otimes>\<^sub>u c |b c. True}\<close>
-    apply (rule update_basis_tensor'[where A=UNIV and B=UNIV])
+proof (rule register_eqI[where A=\<open>{a\<otimes>\<^sub>ub\<otimes>\<^sub>uc| a b c. True}\<close>])
+  have \<open>update_base TYPE('d) {b \<otimes>\<^sub>u c |b c. True}\<close>
+    apply (rule update_base_tensor'[where A=UNIV and B=UNIV])
     by auto
-  then show \<open>update_basis TYPE('d) {a \<otimes>\<^sub>u b \<otimes>\<^sub>u c |a b c. True}\<close>
-    apply (rule_tac update_basis_tensor'[where A=UNIV and B=\<open>{b\<otimes>\<^sub>uc| b c. True}\<close>])
+  then show \<open>update_base TYPE('d) {a \<otimes>\<^sub>u b \<otimes>\<^sub>u c |a b c. True}\<close>
+    apply (rule_tac update_base_tensor'[where A=UNIV and B=\<open>{b\<otimes>\<^sub>uc| b c. True}\<close>])
     by auto
-  show \<open>update_hom F\<close> \<open>update_hom G\<close> by auto
+  show \<open>preregister F\<close> \<open>preregister G\<close> by auto
   show \<open>x \<in> {a \<otimes>\<^sub>u b \<otimes>\<^sub>u c |a b c. True} \<Longrightarrow> F x = G x\<close> for x
     using assms(3) by auto
 qed
 
 lemma tensor_extensionality3': 
   fixes F G :: \<open>(('a::domain\<times>'b::domain)\<times>'c::domain) update \<Rightarrow> 'd::domain update\<close>
-  assumes [simp]: \<open>lvalue F\<close> \<open>lvalue G\<close>
+  assumes [simp]: \<open>register F\<close> \<open>register G\<close>
   assumes "\<And>f g h. F ((f \<otimes>\<^sub>u g) \<otimes>\<^sub>u h) = G ((f \<otimes>\<^sub>u g) \<otimes>\<^sub>u h)"
   shows "F = G"
-proof (rule lvalue_eqI[where A=\<open>{(a\<otimes>\<^sub>ub)\<otimes>\<^sub>uc| a b c. True}\<close>])
-  have \<open>update_basis TYPE('d) {a \<otimes>\<^sub>u b | a b. True}\<close>
-    apply (rule update_basis_tensor'[where A=UNIV and B=UNIV])
+proof (rule register_eqI[where A=\<open>{(a\<otimes>\<^sub>ub)\<otimes>\<^sub>uc| a b c. True}\<close>])
+  have \<open>update_base TYPE('d) {a \<otimes>\<^sub>u b | a b. True}\<close>
+    apply (rule update_base_tensor'[where A=UNIV and B=UNIV])
     by auto
-  then show \<open>update_basis TYPE('d) {(a \<otimes>\<^sub>u b) \<otimes>\<^sub>u c |a b c. True}\<close>
-    apply (rule_tac update_basis_tensor'[where B=UNIV and A=\<open>{a\<otimes>\<^sub>ub| a b. True}\<close>])
+  then show \<open>update_base TYPE('d) {(a \<otimes>\<^sub>u b) \<otimes>\<^sub>u c |a b c. True}\<close>
+    apply (rule_tac update_base_tensor'[where B=UNIV and A=\<open>{a\<otimes>\<^sub>ub| a b. True}\<close>])
     by auto
-  show \<open>update_hom F\<close> \<open>update_hom G\<close> by auto
+  show \<open>preregister F\<close> \<open>preregister G\<close> by auto
   show \<open>x \<in> {(a \<otimes>\<^sub>u b) \<otimes>\<^sub>u c |a b c. True} \<Longrightarrow> F x = G x\<close> for x
     using assms(3) by auto
 qed
@@ -160,15 +159,15 @@ subsection \<open>Pairs and compatibility\<close>
 
 definition compatible :: \<open>('a::domain update \<Rightarrow> 'c::domain update)
                        \<Rightarrow> ('b::domain update \<Rightarrow> 'c update) \<Rightarrow> bool\<close> where
-  \<open>compatible F G \<longleftrightarrow> lvalue F \<and> lvalue G \<and> (\<forall>a b. F a *\<^sub>u G b = G b *\<^sub>u F a)\<close>
+  \<open>compatible F G \<longleftrightarrow> register F \<and> register G \<and> (\<forall>a b. F a *\<^sub>u G b = G b *\<^sub>u F a)\<close>
 
 lemma compatibleI:
-  assumes "lvalue F" and "lvalue G"
+  assumes "register F" and "register G"
   assumes \<open>\<And>a b. (F a) *\<^sub>u (G b) = (G b) *\<^sub>u (F a)\<close>
   shows "compatible F G"
   using assms unfolding compatible_def by simp
 
-lemma swap_lvalues:
+lemma swap_registers:
   assumes "compatible R S"
   shows "R a *\<^sub>u S b = S b *\<^sub>u R a"
   using assms unfolding compatible_def by metis
@@ -176,45 +175,45 @@ lemma swap_lvalues:
 lemma compatible_sym: "compatible x y \<Longrightarrow> compatible y x"
   by (simp add: compatible_def)
 
-lemma pair_lvalue[simp]:
+lemma pair_is_register[simp]:
   assumes "compatible F G"
-  shows "lvalue (F; G)"
-  by (metis assms compatible_def lvalue_pair_lvalue)
+  shows "register (F; G)"
+  by (metis assms compatible_def register_pair_is_register)
 
-lemma lvalue_pair_apply:
+lemma register_pair_apply:
   assumes \<open>compatible F G\<close>
   shows \<open>(F; G) (a \<otimes>\<^sub>u b) = (F a) *\<^sub>u (G b)\<close>
-  apply (rule lvalue_pair_apply)
+  apply (rule register_pair_apply)
   using assms unfolding compatible_def by metis+
 
-lemma lvalue_pair_apply':
+lemma register_pair_apply':
   assumes \<open>compatible F G\<close>
   shows \<open>(F; G) (a \<otimes>\<^sub>u b) = (G b) *\<^sub>u (F a)\<close>
-  apply (subst lvalue_pair_apply)
-  using assms by (auto simp: compatible_def intro: lvalue_hom)
+  apply (subst register_pair_apply)
+  using assms by (auto simp: compatible_def intro: register_preregister)
 
 
 
-lemma compatible_comp_left[simp]: "compatible F G \<Longrightarrow> lvalue H \<Longrightarrow> compatible (F \<circ> H) G"
+lemma compatible_comp_left[simp]: "compatible F G \<Longrightarrow> register H \<Longrightarrow> compatible (F \<circ> H) G"
   by (simp add: compatible_def)
 
-lemma compatible_comp_right[simp]: "compatible F G \<Longrightarrow> lvalue H \<Longrightarrow> compatible F (G \<circ> H)"
+lemma compatible_comp_right[simp]: "compatible F G \<Longrightarrow> register H \<Longrightarrow> compatible F (G \<circ> H)"
   by (simp add: compatible_def)
 
 lemma compatible_comp_inner[simp]: 
-  "compatible F G \<Longrightarrow> lvalue H \<Longrightarrow> compatible (H \<circ> F) (H \<circ> G)"
-  by (smt (verit, best) comp_apply compatible_def lvalue_comp lvalue_mult)
+  "compatible F G \<Longrightarrow> register H \<Longrightarrow> compatible (H \<circ> F) (H \<circ> G)"
+  by (smt (verit, best) comp_apply compatible_def register_comp register_mult)
 
-lemma compatible_lvalue1: \<open>compatible F G \<Longrightarrow> lvalue F\<close>
+lemma compatible_register1: \<open>compatible F G \<Longrightarrow> register F\<close>
   by (simp add: compatible_def)
-lemma compatible_lvalue2: \<open>compatible F G \<Longrightarrow> lvalue G\<close>
+lemma compatible_register2: \<open>compatible F G \<Longrightarrow> register G\<close>
   by (simp add: compatible_def)
 
 lemma pair_o_tensor:
-  assumes "compatible A B" and [simp]: \<open>lvalue C\<close> and [simp]: \<open>lvalue D\<close>
+  assumes "compatible A B" and [simp]: \<open>register C\<close> and [simp]: \<open>register D\<close>
   shows "(A; B) o (C \<otimes>\<^sub>h D) = (A o C; B o D)"
   apply (rule tensor_extensionality)
-  using assms by (simp_all add: tensor_update_hom_is_hom lvalue_pair_apply comp_update_hom)
+  using assms by (simp_all add: register_tensor_is_hom register_pair_apply comp_preregister)
 
 lemma compatible_tensor_id_update_left[simp]:
   fixes F :: "'a::domain update \<Rightarrow> 'c::domain update" and G :: "'b::domain update \<Rightarrow> 'c::domain update"
@@ -231,34 +230,34 @@ lemma compatible_tensor_id_update_right[simp]:
   by simp
 
 lemma compatible_tensor_id_update_rl[simp]:
-  assumes "lvalue F" and "lvalue G"
+  assumes "register F" and "register G"
   shows "compatible (\<lambda>a. F a \<otimes>\<^sub>u id_update) (\<lambda>a. id_update \<otimes>\<^sub>u G a)"
   apply (rule compatibleI)
   using assms by (auto simp: tensor_update_mult)
   
 lemma compatible_tensor_id_update_lr[simp]:
-  assumes "lvalue F" and "lvalue G"
+  assumes "register F" and "register G"
   shows "compatible (\<lambda>a. id_update \<otimes>\<^sub>u F a) (\<lambda>a. G a \<otimes>\<^sub>u id_update)"
   apply (rule compatibleI)
   using assms by (auto simp: tensor_update_mult)
 
-lemma lvalue_comp_pair:
-  assumes [simp]: \<open>lvalue F\<close> and [simp]: \<open>compatible G H\<close>
+lemma register_comp_pair:
+  assumes [simp]: \<open>register F\<close> and [simp]: \<open>compatible G H\<close>
   shows "(F o G; F o H) = F o (G; H)"
 proof (rule tensor_extensionality)
-  show \<open>update_hom (F \<circ> G;F \<circ> H)\<close> and \<open>update_hom (F \<circ> (G;H))\<close>
+  show \<open>preregister (F \<circ> G;F \<circ> H)\<close> and \<open>preregister (F \<circ> (G;H))\<close>
     by simp_all
 
   have [simp]: \<open>compatible (F o G) (F o H)\<close>
     apply (rule compatible_comp_inner, simp)
     by simp
-  then have [simp]: \<open>lvalue (F \<circ> G)\<close> \<open>lvalue (F \<circ> H)\<close>
+  then have [simp]: \<open>register (F \<circ> G)\<close> \<open>register (F \<circ> H)\<close>
     unfolding compatible_def by auto
-  from assms have [simp]: \<open>lvalue G\<close> \<open>lvalue H\<close>
+  from assms have [simp]: \<open>register G\<close> \<open>register H\<close>
     unfolding compatible_def by auto
   fix a b
   show \<open>(F \<circ> G;F \<circ> H) (a \<otimes>\<^sub>u b) = (F \<circ> (G;H)) (a \<otimes>\<^sub>u b)\<close>
-    by (auto simp: lvalue_pair_apply lvalue_mult tensor_update_mult)
+    by (auto simp: register_pair_apply register_mult tensor_update_mult)
 qed
 
 subsection \<open>Fst and Snd\<close>
@@ -266,11 +265,11 @@ subsection \<open>Fst and Snd\<close>
 definition Fst where \<open>Fst a = a \<otimes>\<^sub>u id_update\<close>
 definition Snd where \<open>Snd a = id_update \<otimes>\<^sub>u a\<close>
 
-lemma lvalue_Fst[simp]: \<open>lvalue Fst\<close>
-  unfolding Fst_def by (rule lvalue_tensor_left)
+lemma register_Fst[simp]: \<open>register Fst\<close>
+  unfolding Fst_def by (rule register_tensor_left)
 
-lemma lvalue_Snd[simp]: \<open>lvalue Snd\<close>
-  unfolding Snd_def by (rule lvalue_tensor_right)
+lemma register_Snd[simp]: \<open>register Snd\<close>
+  unfolding Snd_def by (rule register_tensor_right)
 
 lemma compatible_Fst_Snd[simp]: \<open>compatible Fst Snd\<close>
   apply (rule compatibleI, simp, simp)
@@ -282,50 +281,50 @@ definition \<open>swap = (Snd; Fst)\<close>
 
 lemma swap_apply[simp]: "swap (a \<otimes>\<^sub>u b) = (b \<otimes>\<^sub>u a)"
   unfolding swap_def
-  by (simp add: Axioms.lvalue_pair_apply Fst_def Snd_def tensor_update_mult) 
+  by (simp add: Axioms.register_pair_apply Fst_def Snd_def tensor_update_mult) 
 
 lemma swap_o_Fst: "swap o Fst = Snd"
   by (auto simp add: Fst_def Snd_def)
 lemma swap_o_Snd: "swap o Snd = Fst"
   by (auto simp add: Fst_def Snd_def)
 
-lemma lvalue_swap[simp]: \<open>lvalue swap\<close>
+lemma register_swap[simp]: \<open>register swap\<close>
   by (simp add: swap_def)
 
 lemma pair_Fst_Snd: \<open>(Fst; Snd) = id\<close>
   apply (rule tensor_extensionality)
-  by (simp_all add: lvalue_pair_apply Fst_def Snd_def tensor_update_mult)
+  by (simp_all add: register_pair_apply Fst_def Snd_def tensor_update_mult)
 
 (* lemma pair_Snd_Fst: \<open>(Snd; Fst) = swap\<close>
   apply (rule tensor_extensionality)
-  by (simp_all add: lvalue_pair_apply Fst_def Snd_def tensor_update_mult) *)
+  by (simp_all add: register_pair_apply Fst_def Snd_def tensor_update_mult) *)
 
-lemma lvalue_Fst_lvalue_Snd[simp]: 
-  assumes \<open>lvalue F\<close>
+lemma register_Fst_register_Snd[simp]: 
+  assumes \<open>register F\<close>
   shows \<open>(F o Fst; F o Snd) = F\<close>
   apply (rule tensor_extensionality)
-  using assms by (auto simp: lvalue_pair_apply Fst_def Snd_def lvalue_mult tensor_update_mult)
+  using assms by (auto simp: register_pair_apply Fst_def Snd_def register_mult tensor_update_mult)
 
-lemma lvalue_Snd_lvalue_Fst[simp]: 
-  assumes \<open>lvalue F\<close>
+lemma register_Snd_register_Fst[simp]: 
+  assumes \<open>register F\<close>
   shows \<open>(F o Snd; F o Fst) = F o swap\<close>
   apply (rule tensor_extensionality)
-  using assms by (auto simp: lvalue_pair_apply Fst_def Snd_def lvalue_mult tensor_update_mult lvalue_swap)
+  using assms by (auto simp: register_pair_apply Fst_def Snd_def register_mult tensor_update_mult)
 
 
 lemma compatible3[simp]:
   assumes [simp]: "compatible F G" and "compatible G H" and "compatible F H"
   shows "compatible (F; G) H"
 proof (rule compatibleI)
-  have [simp]: \<open>lvalue F\<close> \<open>lvalue G\<close> \<open>lvalue H\<close>
+  have [simp]: \<open>register F\<close> \<open>register G\<close> \<open>register H\<close>
     using assms compatible_def by auto
-  then have [simp]: \<open>update_hom F\<close> \<open>update_hom G\<close> \<open>update_hom H\<close>
-    using lvalue_hom by blast+
-  have [simp]: \<open>update_hom (\<lambda>a. (F;G) a *\<^sub>u z)\<close> for z
-    apply (rule comp_update_hom[unfolded o_def, of \<open>(F;G)\<close>])
+  then have [simp]: \<open>preregister F\<close> \<open>preregister G\<close> \<open>preregister H\<close>
+    using register_preregister by blast+
+  have [simp]: \<open>preregister (\<lambda>a. (F;G) a *\<^sub>u z)\<close> for z
+    apply (rule comp_preregister[unfolded o_def, of \<open>(F;G)\<close>])
     by simp_all
-  have [simp]: \<open>update_hom (\<lambda>a. z *\<^sub>u (F;G) a)\<close> for z
-    apply (rule comp_update_hom[unfolded o_def, of \<open>(F;G)\<close>])
+  have [simp]: \<open>preregister (\<lambda>a. z *\<^sub>u (F;G) a)\<close> for z
+    apply (rule comp_preregister[unfolded o_def, of \<open>(F;G)\<close>])
     by simp_all
   have "(F; G) (f \<otimes>\<^sub>u g) *\<^sub>u H h = H h *\<^sub>u (F; G) (f \<otimes>\<^sub>u g)" for f g h
   proof -
@@ -334,18 +333,18 @@ proof (rule compatibleI)
     have GH: "G g *\<^sub>u H h = H h *\<^sub>u G g"
       using assms compatible_def by metis
     have \<open>(F; G) (f \<otimes>\<^sub>u g) *\<^sub>u (H h) = F f *\<^sub>u G g *\<^sub>u H h\<close>
-      using \<open>compatible F G\<close> by (subst lvalue_pair_apply, auto)
+      using \<open>compatible F G\<close> by (subst register_pair_apply, auto)
     also have \<open>\<dots> = H h *\<^sub>u F f *\<^sub>u G g\<close>
       using FH GH by (metis comp_update_assoc)
     also have \<open>\<dots> = H h *\<^sub>u (F; G) (f \<otimes>\<^sub>u g)\<close>
-      using \<open>compatible F G\<close> by (subst lvalue_pair_apply, auto simp: comp_update_assoc)
+      using \<open>compatible F G\<close> by (subst register_pair_apply, auto simp: comp_update_assoc)
     finally show ?thesis
       by -
   qed
   then show "(F; G) fg *\<^sub>u (H h) = (H h) *\<^sub>u (F; G) fg" for fg h
     apply (rule_tac tensor_extensionality[THEN fun_cong])
     by auto
-  show "lvalue H" and  "lvalue (F; G)"
+  show "register H" and  "register (F; G)"
     by simp_all
 qed
 
@@ -360,19 +359,19 @@ lemma pair_o_swap[simp]:
   assumes [simp]: "compatible A B"
   shows "(A; B) o swap = (B; A)"
 proof (rule tensor_extensionality)
-  have [simp]: "update_hom A" "update_hom B"
-    apply (metis (no_types, hide_lams) assms compatible_lvalue1 lvalue_hom)
-    by (metis (full_types) assms compatible_lvalue2 lvalue_hom)
-  then show \<open>update_hom ((A; B) \<circ> swap)\<close>
-    by (simp add: assms lvalue_swap)
-  show \<open>update_hom (B; A)\<close>
-    by (metis (no_types, lifting) assms compatible_sym lvalue_hom pair_lvalue)
+  have [simp]: "preregister A" "preregister B"
+    apply (metis (no_types, hide_lams) assms compatible_register1 register_preregister)
+    by (metis (full_types) assms compatible_register2 register_preregister)
+  then show \<open>preregister ((A; B) \<circ> swap)\<close>
+    by simp
+  show \<open>preregister (B; A)\<close>
+    by (metis (no_types, lifting) assms compatible_sym register_preregister pair_is_register)
   show \<open>((A; B) \<circ> swap) (a \<otimes>\<^sub>u b) = (B; A) (a \<otimes>\<^sub>u b)\<close> for a b
     (* Without the "only:", we would not need the "apply subst",
        but that proof fails when instantiated in Classical.thy *)
     apply (simp only: o_def swap_apply)
-    apply (subst lvalue_pair_apply, simp)
-    apply (subst lvalue_pair_apply, simp add: compatible_sym)
+    apply (subst register_pair_apply, simp)
+    apply (subst register_pair_apply, simp add: compatible_sym)
     by (metis (no_types, lifting) assms compatible_def)
 qed
 
@@ -381,26 +380,26 @@ subsection \<open>Associativity of the tensor product\<close>
 definition assoc :: \<open>(('a::domain\<times>'b::domain)\<times>'c::domain) update \<Rightarrow> ('a\<times>('b\<times>'c)) update\<close> where 
   \<open>assoc = ((Fst; Snd o Fst); Snd o Snd)\<close>
 
-lemma assoc_is_hom[simp]: \<open>update_hom assoc\<close>
+lemma assoc_is_hom[simp]: \<open>preregister assoc\<close>
   by (auto simp: assoc_def)
 
 lemma assoc_apply: \<open>assoc ((a \<otimes>\<^sub>u b) \<otimes>\<^sub>u c) = (a \<otimes>\<^sub>u (b \<otimes>\<^sub>u c))\<close>
-  by (auto simp: assoc_def lvalue_pair_apply Fst_def Snd_def tensor_update_mult)
+  by (auto simp: assoc_def register_pair_apply Fst_def Snd_def tensor_update_mult)
 
 definition assoc' :: \<open>('a\<times>('b\<times>'c)) update \<Rightarrow> (('a::domain\<times>'b::domain)\<times>'c::domain) update\<close> where 
   \<open>assoc' = (Fst o Fst; (Fst o Snd; Snd))\<close>
 
-lemma assoc'_is_hom[simp]: \<open>update_hom assoc'\<close>
+lemma assoc'_is_hom[simp]: \<open>preregister assoc'\<close>
   by (auto simp: assoc'_def)
 
 lemma assoc'_apply: \<open>assoc' (a \<otimes>\<^sub>u (b \<otimes>\<^sub>u c)) =  ((a \<otimes>\<^sub>u b) \<otimes>\<^sub>u c)\<close>
-  by (auto simp: assoc'_def lvalue_pair_apply Fst_def Snd_def tensor_update_mult)
+  by (auto simp: assoc'_def register_pair_apply Fst_def Snd_def tensor_update_mult)
 
-lemma lvalue_assoc[simp]: \<open>lvalue assoc\<close>
+lemma register_assoc[simp]: \<open>register assoc\<close>
   unfolding assoc_def
   by force
 
-lemma lvalue_assoc'[simp]: \<open>lvalue assoc'\<close>
+lemma register_assoc'[simp]: \<open>register assoc'\<close>
   unfolding assoc'_def 
   by force
 
@@ -408,38 +407,38 @@ lemma pair_o_assoc[simp]:
   assumes [simp]: \<open>compatible F G\<close> \<open>compatible G H\<close> \<open>compatible F H\<close>
   shows \<open>(F; (G; H)) \<circ> assoc = ((F; G); H)\<close>
 proof (rule tensor_extensionality3')
-  show \<open>lvalue ((F; (G; H)) \<circ> assoc)\<close>
+  show \<open>register ((F; (G; H)) \<circ> assoc)\<close>
     by simp
-  show \<open>lvalue ((F; G); H)\<close>
+  show \<open>register ((F; G); H)\<close>
     by simp
   show \<open>((F; (G; H)) \<circ> assoc) ((f \<otimes>\<^sub>u g) \<otimes>\<^sub>u h) = ((F; G); H) ((f \<otimes>\<^sub>u g) \<otimes>\<^sub>u h)\<close> for f g h
-    by (simp add: lvalue_pair_apply assoc_apply comp_update_assoc)
+    by (simp add: register_pair_apply assoc_apply comp_update_assoc)
 qed
 
 lemma pair_o_assoc'[simp]:
   assumes [simp]: \<open>compatible F G\<close> \<open>compatible G H\<close> \<open>compatible F H\<close>
   shows \<open>((F; G); H) \<circ> assoc' = (F; (G; H))\<close>
 proof (rule tensor_extensionality3)
-  show \<open>lvalue (((F; G); H) \<circ> assoc')\<close>
-    by (simp add: lvalue_assoc')
-  show \<open>lvalue (F; (G; H))\<close>
+  show \<open>register (((F; G); H) \<circ> assoc')\<close>
+    by simp
+  show \<open>register (F; (G; H))\<close>
     by simp
   show \<open>(((F; G); H) \<circ> assoc') (f \<otimes>\<^sub>u g \<otimes>\<^sub>u h) = (F; (G; H)) (f \<otimes>\<^sub>u g \<otimes>\<^sub>u h)\<close> for f g h
-    by (simp add: lvalue_pair_apply assoc'_apply comp_update_assoc)
+    by (simp add: register_pair_apply assoc'_apply comp_update_assoc)
 qed
 
 subsection \<open>Compatibility simplification\<close>
 
 (* The simproc compatibility_warn produces helpful warnings for "compatible x y"
    subgoals that are probably unsolvable due to missing declarations of 
-   variable compatibility facts. Same for "lvalue x" subgoals. *)
-simproc_setup "compatibility_warn" ("compatible x y" | "lvalue x") = \<open>
+   variable compatibility facts. Same for "register x" subgoals. *)
+simproc_setup "compatibility_warn" ("compatible x y" | "register x") = \<open>
 let val thy_string = Markup.markup (Theory.get_markup \<^theory>) (Context.theory_name \<^theory>)
 in
 fn m => fn ctxt => fn ct => let
   val (x,y) = case Thm.term_of ct of
                  Const(\<^const_name>\<open>compatible\<close>,_ ) $ x $ y => (x, SOME y)
-               | Const(\<^const_name>\<open>lvalue\<close>,_ ) $ x => (x, NONE)
+               | Const(\<^const_name>\<open>register\<close>,_ ) $ x => (x, NONE)
   val str : string lazy = Lazy.lazy (fn () => Syntax.string_of_term ctxt (Thm.term_of ct))
   fun w msg = warning (msg ^ "\n(Disable these warnings with: using [[simproc del: "^thy_string^".compatibility_warn]])")
   (* val _ = \<^print> (m,ctxt,ct) *)
@@ -466,8 +465,8 @@ fn m => fn ctxt => fn ct => let
             else w ("Simplification subgoal " ^ Lazy.force str ^ " occurred but cannot be solved.\n" ^
                     "Please add assumption/fact  [simp]: \<open>" ^ Lazy.force str ^ "\<close>  somewhere.")
 (*       | (_, NONE) => w ("Simplification subgoal " ^ Lazy.force str ^ 
-                    "\ncannot be reduced to a judgment about a single variable (such as \<open>lvalue x\<close>).\n" ^
-                    "Try adding a simplification rule that breaks it down (such as, e.g., " ^ @{fact lvalue_comp} ^ ").") *)
+                    "\ncannot be reduced to a judgment about a single variable (such as \<open>register x\<close>).\n" ^
+                    "Try adding a simplification rule that breaks it down (such as, e.g., " ^ @{fact register_comp} ^ ").") *)
       | _ => ()
   in NONE end
 end\<close>
@@ -475,7 +474,7 @@ end\<close>
 
 (* Declares the attribute [compatible]. If applied to a conjunction 
    of "compatible x y" facts, it will add all of them to the simplifier
-   (as [simp] does), but additionally add all "lvalue x", "lvalue y" facts. *)
+   (as [simp] does), but additionally add all "register x", "register y" facts. *)
 setup \<open>
 let 
 fun add (thm:thm) results = 
@@ -485,7 +484,7 @@ fun collect thm results = case Thm.concl_of thm of
   Const(\<^const_name>\<open>Trueprop\<close>,_) $ (Const(\<^const_name>\<open>conj\<close>,_) $ _ $ _) => 
     collect (@{thm conjunct1} OF [thm]) (collect (@{thm conjunct2} OF [thm]) results)
   | Const(\<^const_name>\<open>Trueprop\<close>,_) $ (Const(\<^const_name>\<open>compatible\<close>,_) $ _ $ _) =>
-    collect (@{thm compatible_lvalue1} OF [thm]) (collect (@{thm compatible_lvalue2} OF [thm]) (add thm results))
+    collect (@{thm compatible_register1} OF [thm]) (collect (@{thm compatible_register2} OF [thm]) (add thm results))
   | _ => add thm results
 fun declare thm context = let
   val thms = collect thm (Net.empty) |> Net.entries
@@ -493,7 +492,7 @@ fun declare thm context = let
 in
 Attrib.setup \<^binding>\<open>compatible\<close>
  (Scan.succeed (Thm.declaration_attribute declare))
-  "Add 'compatible x y' style rules to simplifier. (Also adds 'lvalue x', 'lvalue y')"
+  "Add 'compatible x y' style rules to simplifier. (Also adds 'register x', 'register y')"
 end
 \<close>
 
@@ -504,14 +503,14 @@ subsection \<open>Notation\<close>
 no_notation comp_update (infixl "*\<^sub>u" 55)
 no_notation tensor_update (infixr "\<otimes>\<^sub>u" 70)
 
-bundle lvalue_notation begin
-notation tensor_update_hom (infixr "\<otimes>\<^sub>h" 70)
-notation lvalue_pair ("'(_;_')")
+bundle register_notation begin
+notation register_tensor (infixr "\<otimes>\<^sub>h" 70)
+notation register_pair ("'(_;_')")
 end
 
-bundle no_lvalue_notation begin
-no_notation tensor_update_hom (infixr "\<otimes>\<^sub>h" 70)
-no_notation lvalue_pair ("'(_;_')")
+bundle no_register_notation begin
+no_notation register_tensor (infixr "\<otimes>\<^sub>h" 70)
+no_notation register_pair ("'(_;_')")
 end
 
 end
