Axioms.thy
@@ -1,4 +1,4 @@
-section \<open>Axioms of lvalues\<close>
+section \<open>Axioms of registerss\<close>
 
 theory Axioms
   imports Main
@@ -15,19 +15,19 @@ axiomatization id_update :: "'a::domain update" where
   id_update_left: "comp_update id_update a = a" and
   id_update_right: "comp_update a id_update = a"
 
-axiomatization update_hom :: \<open>('a::domain update \<Rightarrow> 'b::domain update) \<Rightarrow> bool\<close>
+axiomatization preregister :: \<open>('a::domain update \<Rightarrow> 'b::domain update) \<Rightarrow> bool\<close>
 axiomatization where
-  comp_update_hom: "update_hom F \<Longrightarrow> update_hom G \<Longrightarrow> update_hom (G \<circ> F)" and
-  id_update_hom: \<open>update_hom id\<close>
+  comp_preregister: "preregister F \<Longrightarrow> preregister G \<Longrightarrow> preregister (G \<circ> F)" and
+  id_preregister: \<open>preregister id\<close>
 for F :: \<open>'a::domain update \<Rightarrow> 'b::domain update\<close> and G :: \<open>'b update \<Rightarrow> 'c::domain update\<close>
 
 axiomatization where
-  update_hom_mult_right: \<open>update_hom (\<lambda>a. comp_update a z)\<close> and
-  update_hom_mult_left: \<open>update_hom (\<lambda>a. comp_update z a)\<close>
+  preregister_mult_right: \<open>preregister (\<lambda>a. comp_update a z)\<close> and
+  preregister_mult_left: \<open>preregister (\<lambda>a. comp_update z a)\<close>
     for z :: "'a::domain update"
 
 axiomatization tensor_update :: \<open>'a::domain update \<Rightarrow> 'b::domain update \<Rightarrow> ('a\<times>'b) update\<close> 
-    where tensor_extensionality: "update_hom F \<Longrightarrow> update_hom G \<Longrightarrow> (\<And>a b. F (tensor_update a b) = G (tensor_update a b)) \<Longrightarrow> F = G"
+    where tensor_extensionality: "preregister F \<Longrightarrow> preregister G \<Longrightarrow> (\<And>a b. F (tensor_update a b) = G (tensor_update a b)) \<Longrightarrow> F = G"
     for F G :: \<open>('a\<times>'b) update \<Rightarrow> 'c::domain update\<close>
 
 axiomatization where tensor_update_mult: \<open>comp_update (tensor_update a c) (tensor_update b d) = tensor_update (comp_update a b) (comp_update c d)\<close>
@@ -35,27 +35,27 @@ axiomatization where tensor_update_mult: \<open>comp_update (tensor_update a c) 
 
 
 axiomatization where
-  update_hom_tensor_left_is_hom: "update_hom (tensor_update a :: 'b::domain update \<Rightarrow> _)" and
-  update_hom_tensor_right_is_hom: "update_hom (\<lambda>a::'a::domain update. tensor_update a b)"
+  preregister_tensor_left: "preregister (tensor_update a :: 'b::domain update \<Rightarrow> _)" and
+  preregister_tensor_right: "preregister (\<lambda>a::'a::domain update. tensor_update a b)"
   for a :: "'a::domain update" and b :: "'b::domain update"
 
-axiomatization lvalue :: \<open>('a update \<Rightarrow> 'b update) \<Rightarrow> bool\<close>
+axiomatization register :: \<open>('a update \<Rightarrow> 'b update) \<Rightarrow> bool\<close>
 axiomatization where
-  lvalue_hom: "lvalue F \<Longrightarrow> update_hom F" and
-  lvalue_comp: "lvalue F \<Longrightarrow> lvalue G \<Longrightarrow> lvalue (G \<circ> F)"  and
-  lvalue_mult: "lvalue F \<Longrightarrow> comp_update (F a) (F b) = F (comp_update a b)" and
-  lvalue_of_id: \<open>lvalue F \<Longrightarrow> F id_update = id_update\<close>
+  register_preregister: "register F \<Longrightarrow> preregister F" and
+  register_comp: "register F \<Longrightarrow> register G \<Longrightarrow> register (G \<circ> F)"  and
+  register_mult: "register F \<Longrightarrow> comp_update (F a) (F b) = F (comp_update a b)" and
+  register_id: \<open>register F \<Longrightarrow> F id_update = id_update\<close>
 for F :: "'a::domain update \<Rightarrow> 'b::domain update" and G :: "'b update \<Rightarrow> 'c::domain update" 
 
-axiomatization where lvalue_tensor_left: \<open>lvalue (\<lambda>a. tensor_update a id_update)\<close>
-axiomatization where lvalue_tensor_right: \<open>lvalue (\<lambda>a. tensor_update id_update a)\<close>
+axiomatization where register_tensor_left: \<open>register (\<lambda>a. tensor_update a id_update)\<close>
+axiomatization where register_tensor_right: \<open>register (\<lambda>a. tensor_update id_update a)\<close>
 
-axiomatization lvalue_pair ::
+axiomatization register_pair ::
   \<open>('a::domain update \<Rightarrow> 'c::domain update) \<Rightarrow> ('b::domain update \<Rightarrow> 'c update)
          \<Rightarrow> (('a\<times>'b) update \<Rightarrow> 'c update)\<close> where
-  lvalue_pair_lvalue: \<open>lvalue F \<Longrightarrow> lvalue G \<Longrightarrow> (\<And>a b. comp_update (F a) (G b) = comp_update (G b) (F a))
-       \<Longrightarrow> lvalue (lvalue_pair F G)\<close> and
-  lvalue_pair_apply: \<open>lvalue F \<Longrightarrow> lvalue G \<Longrightarrow> (\<And>a b. comp_update (F a) (G b) = comp_update (G b) (F a))
-       \<Longrightarrow> (lvalue_pair F G) (tensor_update a b) = comp_update (F a) (G b)\<close>
+  register_pair_is_register: \<open>register F \<Longrightarrow> register G \<Longrightarrow> (\<And>a b. comp_update (F a) (G b) = comp_update (G b) (F a))
+       \<Longrightarrow> register (register_pair F G)\<close> and
+  register_pair_apply: \<open>register F \<Longrightarrow> register G \<Longrightarrow> (\<And>a b. comp_update (F a) (G b) = comp_update (G b) (F a))
+       \<Longrightarrow> (register_pair F G) (tensor_update a b) = comp_update (F a) (G b)\<close>
 
 end
