Quantum_Extra.thy
@@ -1,4 +1,4 @@
-section \<open>Derived facts about quantum lvalues\<close>
+section \<open>Derived facts about quantum registers\<close>
 
 theory Quantum_Extra
   imports
@@ -12,26 +12,26 @@ begin
 no_notation meet (infixl "\<sqinter>\<index>" 70)
 no_notation Group.mult (infixl "\<otimes>\<index>" 70)
 no_notation Order.top ("\<top>\<index>")
-unbundle lvalue_notation
+unbundle register_notation
 unbundle cblinfun_notation
 
-lemma lvalue_id[simp]: \<open>lvalue (\<lambda>x. x)\<close>
-  by (metis (mono_tags, lifting) complex_vector.module_hom_ident lvalue_def)
+lemma register_id[simp]: \<open>register (\<lambda>x. x)\<close>
+  by (metis (mono_tags, lifting) complex_vector.module_hom_ident register_def)
 
-lemma lvalue_id'[simp]: \<open>lvalue id\<close>
+lemma register_id'[simp]: \<open>register id\<close>
   by (simp add: id_def)
 
-lemma lvalue_projector:
-  assumes "lvalue F"
+lemma register_projector:
+  assumes "register F"
   assumes "isProjector a"
   shows "isProjector (F a)"
-  using assms unfolding lvalue_def isProjector_algebraic by metis
+  using assms unfolding register_def isProjector_algebraic by metis
 
-lemma lvalue_unitary:
-  assumes "lvalue F"
+lemma register_unitary:
+  assumes "register F"
   assumes "unitary a"
   shows "unitary (F a)"
-  using assms by (smt (verit, best) lvalue_def unitary_def)
+  using assms by (smt (verit, best) register_def unitary_def)
 
 lemma compatible_proj_intersect:
   (* I think this also holds without isProjector, but my proof idea uses the Penrose-Moore 
@@ -40,7 +40,7 @@ lemma compatible_proj_intersect:
   shows "(R a *\<^sub>S \<top>) \<sqinter> (S b *\<^sub>S \<top>) = ((R a o\<^sub>C\<^sub>L S b) *\<^sub>S \<top>)"
 proof (rule antisym)
   have "((R a o\<^sub>C\<^sub>L S b) *\<^sub>S \<top>) \<le> (S b *\<^sub>S \<top>)"
-    apply (subst swap_lvalues[OF assms(1)])
+    apply (subst swap_registers[OF assms(1)])
     by (auto simp: cblinfun_apply_assoc_subspace intro!: applyOpSpace_mono)
   moreover have "((R a o\<^sub>C\<^sub>L S b) *\<^sub>S \<top>) \<le> (R a *\<^sub>S \<top>)"
     by (auto simp: cblinfun_apply_assoc_subspace intro!: applyOpSpace_mono)
@@ -48,9 +48,9 @@ proof (rule antisym)
     by auto
 
   have "isProjector (R a)"
-    using assms(1) assms(2) compatible_lvalue1 lvalue_projector by blast
+    using assms(1) assms(2) compatible_register1 register_projector by blast
   have "isProjector (S b)"
-    using assms(1) assms(3) compatible_lvalue2 lvalue_projector by blast
+    using assms(1) assms(3) compatible_register2 register_projector by blast
   show \<open>(R a *\<^sub>S \<top>) \<sqinter> (S b *\<^sub>S \<top>) \<le> (R a o\<^sub>C\<^sub>L S b) *\<^sub>S \<top>\<close>
   proof (unfold less_eq_ccsubspace.rep_eq, rule)
     fix \<psi>
@@ -78,11 +78,11 @@ lemma compatible_proj_mult:
   using [[simproc del: Laws_Quantum.compatibility_warn]]
   using assms unfolding isProjector_algebraic compatible_def
   apply auto
-  apply (metis (no_types, lifting) cblinfun_apply_assoc lvalue_mult)
-  by (simp add: assms(2) assms(3) isProjector_D2 lvalue_projector)
+  apply (metis (no_types, lifting) cblinfun_apply_assoc register_mult)
+  by (simp add: assms(2) assms(3) isProjector_D2 register_projector)
 
-lemma unitary_sandwich_lvalue: \<open>unitary a \<Longrightarrow> lvalue (sandwich a)\<close>
-  unfolding lvalue_def sandwich_def
+lemma unitary_sandwich_register: \<open>unitary a \<Longrightarrow> register (sandwich a)\<close>
+  unfolding register_def sandwich_def
   by (smt (z3) adjoint_twice assoc_left(1) cblinfun_apply_dist1 cblinfun_apply_dist2 clinearI op_scalar_op scalar_op_op times_adjoint times_idOp2 unitary_def)
 
 lemma sandwich_tensor: 
@@ -90,20 +90,20 @@ lemma sandwich_tensor:
   assumes \<open>unitary a\<close> \<open>unitary b\<close>
   shows "sandwich (a \<otimes>\<^sub>o b) = sandwich a \<otimes>\<^sub>h sandwich b"
   apply (rule tensor_extensionality)
-  by (auto simp: unitary_sandwich_lvalue assms sandwich_def tensor_update_hom_is_hom comp_tensor_op tensor_op_adjoint)
+  by (auto simp: unitary_sandwich_register assms sandwich_def register_tensor_is_hom comp_tensor_op tensor_op_adjoint)
 
 lemma sandwich_grow_left: 
   fixes a :: \<open>'a::finite ell2 \<Rightarrow>\<^sub>C\<^sub>L 'a ell2\<close>
   assumes "unitary a"
   shows "sandwich a \<otimes>\<^sub>h id = sandwich (a \<otimes>\<^sub>o idOp)"
-  by (simp add: unitary_sandwich_lvalue assms sandwich_tensor sandwich_id)
+  by (simp add: unitary_sandwich_register assms sandwich_tensor sandwich_id)
 
-lemma lvalue_sandwich: \<open>lvalue F \<Longrightarrow> F (sandwich a b) = sandwich (F a) (F b)\<close>
-  by (smt (verit, del_insts) lvalue_def sandwich_def)
+lemma register_sandwich: \<open>register F \<Longrightarrow> F (sandwich a b) = sandwich (F a) (F b)\<close>
+  by (smt (verit, del_insts) register_def sandwich_def)
 
 lemma assoc_ell2_sandwich: \<open>assoc = sandwich assoc_ell2\<close>
   apply (rule tensor_extensionality3')
-    apply (simp_all add: unitary_sandwich_lvalue)[2]
+    apply (simp_all add: unitary_sandwich_register)[2]
   apply (rule equal_ket)
   apply (case_tac x)
   by (simp add: sandwich_def assoc_apply times_applyOp tensor_op_ell2 assoc_ell2_tensor assoc_ell2'_tensor
@@ -111,7 +111,7 @@ lemma assoc_ell2_sandwich: \<open>assoc = sandwich assoc_ell2\<close>
 
 lemma assoc_ell2'_sandwich: \<open>assoc' = sandwich assoc_ell2'\<close>
   apply (rule tensor_extensionality3)
-    apply (simp_all add: unitary_sandwich_lvalue)[2]
+    apply (simp_all add: unitary_sandwich_register)[2]
   apply (rule equal_ket)
   apply (case_tac x)
   by (simp add: sandwich_def assoc'_apply times_applyOp tensor_op_ell2 assoc_ell2_tensor assoc_ell2'_tensor 
@@ -128,27 +128,27 @@ lemma id_tensor_sandwich:
   assumes "unitary a"
   shows "id \<otimes>\<^sub>h sandwich a = sandwich (idOp \<otimes>\<^sub>o a)"
   apply (rule tensor_extensionality) 
-  using assms by (auto simp: tensor_update_hom_is_hom comp_tensor_op sandwich_def tensor_op_adjoint unitary_sandwich_lvalue)
+  using assms by (auto simp: register_tensor_is_hom comp_tensor_op sandwich_def tensor_op_adjoint unitary_sandwich_register)
 
 lemma compatible_selfbutter_join:
   assumes [compatible]: "compatible R S"
   shows "R (selfbutter \<psi>) o\<^sub>C\<^sub>L S (selfbutter \<phi>) = (R; S) (selfbutter (\<psi> \<otimes>\<^sub>s \<phi>))"
-  apply (subst lvalue_pair_apply[symmetric, where F=R and G=S])
+  apply (subst register_pair_apply[symmetric, where F=R and G=S])
   using assms by auto
 
 definition empty_var :: \<open>'a::{CARD_1,enum} update \<Rightarrow> 'b::finite update\<close> where
   "empty_var a = one_dim_isom a *\<^sub>C idOp"
 
-lemma lvalue_empty_var[simp]: \<open>lvalue empty_var\<close>
-  unfolding lvalue_def empty_var_def
+lemma register_empty_var[simp]: \<open>register empty_var\<close>
+  unfolding register_def empty_var_def
   by (auto simp add: clinearI scaleC_left.add)
 
-lemma empty_var_compatible[simp]: \<open>lvalue X \<Longrightarrow> compatible empty_var X\<close>
+lemma empty_var_compatible[simp]: \<open>register X \<Longrightarrow> compatible empty_var X\<close>
   apply (rule compatibleI)
   using [[simproc del: Laws_Quantum.compatibility_warn]]
   by (auto simp: empty_var_def)
 
-lemma empty_var_compatible'[simp]: \<open>lvalue X \<Longrightarrow> compatible X empty_var\<close>
+lemma empty_var_compatible'[simp]: \<open>register X \<Longrightarrow> compatible X empty_var\<close>
   using compatible_sym empty_var_compatible by blast
 
 end
